MinmalWk.lean
@@ -1,0 +1,106 @@
+inductive RawWk: Type 0 where
+  | id: RawWk
+  | step: RawWk -> RawWk
+  | lift: RawWk -> RawWk
+
+@[simp] def raw_wk_comp: RawWk -> RawWk -> RawWk
+    | RawWk.id, σ => σ
+    | RawWk.step ρ, σ => RawWk.step (raw_wk_comp ρ σ)
+    | RawWk.lift ρ, RawWk.id => RawWk.lift ρ
+    | RawWk.lift ρ, RawWk.step σ => RawWk.step (raw_wk_comp ρ σ)
+    | RawWk.lift ρ, RawWk.lift σ => RawWk.lift (raw_wk_comp ρ σ)
+
+theorem raw_wk_comp_id_left_id {ρ: RawWk}: raw_wk_comp RawWk.id ρ = ρ := rfl
+
+@[simp] theorem raw_wk_comp_id_right_id: {ρ: RawWk} -> raw_wk_comp ρ RawWk.id = ρ
+  | RawWk.id => rfl
+  | RawWk.lift ρ => rfl
+  | RawWk.step ρ => by {
+    simp
+    apply raw_wk_comp_id_right_id
+  }
+
+@[simp] theorem raw_wk_comp_assoc: {ρ σ τ: RawWk} -> 
+  raw_wk_comp (raw_wk_comp ρ σ) τ = raw_wk_comp ρ (raw_wk_comp σ τ)
+  | RawWk.id, _, _ => rfl
+  | _, RawWk.id, _ => by simp
+  | _, _, RawWk.id => by simp
+  | RawWk.step ρ, _, _ => by {
+    simp
+    apply raw_wk_comp_assoc
+  }
+  | RawWk.lift ρ, RawWk.step σ, _ => by {
+    simp
+    apply raw_wk_comp_assoc
+  }
+  | RawWk.lift ρ, RawWk.lift σ, RawWk.step τ => by {
+    simp
+    apply raw_wk_comp_assoc
+  }
+  | RawWk.lift ρ, RawWk.lift σ, RawWk.lift τ => by {
+    simp
+    apply raw_wk_comp_assoc
+  }
+
+@[simp] def raw_wk_var: RawWk -> Nat -> Nat
+  | RawWk.id, n => n
+  | RawWk.step ρ, n => (raw_wk_var ρ n) + 1
+  | RawWk.lift ρ, 0 => 0
+  | RawWk.lift ρ, (n + 1) => (raw_wk_var ρ n) + 1
+
+@[simp] theorem raw_wk_var_comp: (ρ σ: RawWk) -> (n: Nat) ->
+  raw_wk_var ρ (raw_wk_var σ n) = raw_wk_var (raw_wk_comp ρ σ) n
+  | RawWk.id, _, _ => rfl
+  | _, RawWk.id, _ => by { simp }
+  | RawWk.step ρ, _, _ => by { simp; apply raw_wk_var_comp }
+  | RawWk.lift ρ, RawWk.step σ, _ => by { simp; apply raw_wk_var_comp }
+  | RawWk.lift ρ, RawWk.lift σ, 0 => by { simp } 
+  | RawWk.lift ρ, RawWk.lift σ, (n + 1) => by { simp; apply raw_wk_var_comp }  
+
+@[simp] def wk_maps (m n: Nat) (ρ: RawWk): Prop := (l: Nat) -> l < n -> raw_wk_var ρ l < m
+
+theorem wk_maps_id {n: Nat}: wk_maps n n RawWk.id := λ_ => λH => H
+
+theorem wk_maps_step {m n: Nat} {ρ: RawWk}: wk_maps m n ρ -> wk_maps (m + 1) n (RawWk.step ρ) := by {
+  intros Hρ l Hl;
+  simp;
+  apply Nat.succ_lt_succ;
+  apply Hρ;
+  apply Hl
+}
+
+theorem wk_maps_lift {m n: Nat} {ρ: RawWk}: 
+  wk_maps m n ρ -> wk_maps (m + 1) (n + 1) (RawWk.lift ρ) := by {
+  intros Hρ l Hl;
+  cases l with
+  | zero => simp; apply Nat.zero_lt_succ
+  | succ => simp; apply Nat.succ_lt_succ; apply Hρ; apply Nat.lt_of_succ_lt_succ; apply Hl
+}
+
+theorem wk_maps_comp {m n l: Nat} {ρ σ: RawWk}:
+  wk_maps m n ρ -> wk_maps n l σ -> wk_maps m l (raw_wk_comp ρ σ) := by {
+  intros Hρ Hσ l Hl;
+  rw[←raw_wk_var_comp];
+  apply Hρ;
+  apply Hσ;
+  apply Hl
+}
+
+structure Wk (m n: Nat) := (val: RawWk) (p: wk_maps m n val)
+
+@[simp] def Wk.id {n: Nat}: Wk n n := Wk.mk RawWk.id (@wk_maps_id n)
+
+@[simp] def Wk.step {m n: Nat} (ρ: Wk m n): Wk (m + 1) n := 
+  Wk.mk (RawWk.step ρ.val) (wk_maps_step ρ.p)
+
+@[simp] def Wk.lift {m n: Nat} (ρ: Wk m n): Wk (m + 1) (n + 1) := 
+  Wk.mk (RawWk.lift ρ.val) (wk_maps_lift ρ.p)
+
+@[simp] def Wk.comp {m n l: Nat} (ρ: Wk m n) (σ: Wk n l): Wk m l :=
+  Wk.mk (raw_wk_comp ρ.val σ.val) (wk_maps_comp ρ.p σ.p)
+
+theorem wk_comp_assoc {m n l p: Nat} (ρ: Wk m n) (σ: Wk n l) (τ: Wk l p):
+  Wk.comp ρ (Wk.comp σ τ) = Wk.comp (Wk.comp ρ σ) τ := by {
+  simp
+}
+
